

Fokker-Planck representation of stochastic neural fields: derivation, analysis and application to grid cells

Lecture 2 : existence of solutions

Pierre Roux¹ Susanne Solem²

¹Institut Camille Jordan, École Centrale de Lyon.

²Norwegian University of Life Sciences.

Vrije Universiteit Amsterdam,
From Microscopic Dynamics
to Continuum Models



One population model

Recap on the model

$$\frac{\partial \rho}{\partial t} = -\frac{\partial}{\partial s} \left([\Phi_{\bar{\rho}}(\mathbf{x}, t) - s] \rho \right) + \sigma \frac{\partial^2 \rho}{\partial s^2},$$

where $\Phi_{\bar{\rho}}(\mathbf{x}, t)$ is given by

$$\Phi_{\bar{\rho}}(\mathbf{x}, t) = \Phi(W * \bar{\rho}(\mathbf{x}, t) + B),$$

where $B > 0$ is constant and

$$\bar{\rho}(\mathbf{x}, t) = \int_0^\infty s \rho(\mathbf{x}, s, t) \, ds, \quad \Phi_{\bar{\rho}}(\mathbf{x}, t) \rho(\mathbf{x}, 0, t) - \sigma \frac{\partial \rho}{\partial s}(\mathbf{x}, 0, t) = 0.$$

Simplest case

Let's take the simplest possible case : $\Phi \equiv 0$ and $\sigma = 1$. Then,

$$\frac{\partial \rho}{\partial t} = -\frac{\partial}{\partial s}(-s\rho) + \frac{\partial^2 \rho}{\partial s^2}, \quad \frac{\partial \rho}{\partial s}(\mathbf{x}, 0, t) = 0.$$

Simplest case

Let's take the simplest possible case : $\Phi \equiv 0$ and $\sigma = 1$. Then,

$$\frac{\partial \rho}{\partial t} = -\frac{\partial}{\partial s}(-s\rho) + \frac{\partial^2 \rho}{\partial s^2}, \quad \frac{\partial \rho}{\partial s}(\mathbf{x}, 0, t) = 0.$$

Then, use the change of variable $y = e^t s$ and $\tau = \frac{1}{2}(e^{2t} - 1)$. Denoting $\alpha(\tau) = (2\tau + 1)^{-\frac{1}{2}} = e^{-t}$, the function

$$q(x, y, \tau) = \alpha(\tau) \rho\left(x, \underbrace{y\alpha(\tau)}_{=s}, \underbrace{-\log(\alpha(\tau))}_{=t}\right),$$

is solution to

$$\frac{\partial q}{\partial \tau} = \frac{\partial^2 q}{\partial y^2}, \quad \frac{\partial q}{\partial y}(\mathbf{x}, 0, t) = 0.$$

Simplest case

Let's take the simplest possible case : $\Phi \equiv 0$ and $\sigma = 1$. Then,

$$\frac{\partial \rho}{\partial t} = -\frac{\partial}{\partial s}(-s\rho) + \frac{\partial^2 \rho}{\partial s^2}, \quad \frac{\partial \rho}{\partial s}(\mathbf{x}, 0, t) = 0.$$

Then, use the change of variable $y = e^t s$ and $\tau = \frac{1}{2}(e^{2t} - 1)$. Denoting $\alpha(\tau) = (2\tau + 1)^{-\frac{1}{2}} = e^{-t}$, the function

$$q(x, y, \tau) = \alpha(\tau) \rho\left(x, \underbrace{y\alpha(\tau)}_{=s}, \underbrace{-\log(\alpha(\tau))}_{=t}\right),$$

is solution to

$$\frac{\partial q}{\partial \tau} = \frac{\partial^2 q}{\partial y^2}, \quad \frac{\partial q}{\partial y}(\mathbf{x}, 0, t) = 0.$$

This is an easy problem :) .

General case

Coming back to the general case, we can still get $\sigma = 1$ by a linear rescaling.

General case

Coming back to the general case, we can still get $\sigma = 1$ by a linear rescaling.

Let's try again the change of variable $y = e^t s$, $\tau = \frac{1}{2}(e^{2t} - 1)$. Still denoting $\alpha(\tau) = (2\tau + 1)^{-\frac{1}{2}}$ and

$$q(x, y, \tau) = \alpha(\tau) \rho\left(x, y\alpha(\tau), -\log(\alpha(\tau))\right),$$

General case

Coming back to the general case, we can still get $\sigma = 1$ by a linear rescaling.

Let's try again the change of variable $y = e^t s$, $\tau = \frac{1}{2}(e^{2t} - 1)$. Still denoting $\alpha(\tau) = (2\tau + 1)^{-\frac{1}{2}}$ and

$$q(x, y, \tau) = \alpha(\tau) \rho\left(x, y\alpha(\tau), -\log(\alpha(\tau))\right),$$

the function q is now solution at each (x, y, τ) of the problem

$$\frac{\partial q}{\partial \tau} = \frac{\partial^2 q}{\partial y^2} - \Psi(x, \tau) \frac{\partial q}{\partial y}, \quad \Psi(x, \tau) = \Phi_{\bar{\rho}}(x, -\log(\alpha(\tau)))\alpha(\tau), \quad (1)$$

with $\bar{\rho} = \alpha \bar{q}$ and boundary condition

$$\Psi(x, \tau) q(x, 0, \tau) - \frac{\partial q}{\partial y}(x, 0, \tau) = 0.$$

General case

Coming back to the general case, we can still get $\sigma = 1$ by a linear rescaling.

Let's try again the change of variable $y = e^t s$, $\tau = \frac{1}{2}(e^{2t} - 1)$. Still denoting $\alpha(\tau) = (2\tau + 1)^{-\frac{1}{2}}$ and

$$q(x, y, \tau) = \alpha(\tau) \rho\left(x, y\alpha(\tau), -\log(\alpha(\tau))\right),$$

the function q is now solution at each (x, y, τ) of the problem

$$\frac{\partial q}{\partial \tau} = \frac{\partial^2 q}{\partial y^2} - \Psi(x, \tau) \frac{\partial q}{\partial y}, \quad \Psi(x, \tau) = \Phi_{\bar{\rho}}(x, -\log(\alpha(\tau)))\alpha(\tau), \quad (1)$$

with $\bar{\rho} = \alpha \bar{q}$ and boundary condition

$$\Psi(x, \tau) q(x, 0, \tau) - \frac{\partial q}{\partial y}(x, 0, \tau) = 0.$$

This is **not** an easy problem : (

We have

$$\frac{\partial q}{\partial \tau} = \frac{\partial^2 q}{\partial y^2} - \Psi(x, \tau) \frac{\partial q}{\partial y}, \quad \Psi(x, \tau) = \Phi_{\bar{\rho}}(x, -\log(\alpha(\tau)))\alpha(\tau), \quad (2)$$

Let us absorb the drift in the time derivative with the variable

$$z = y - \int_0^\tau \Psi(x, \eta) \, d\eta.$$

Then u solves

$$\frac{\partial u}{\partial \tau} = \frac{\partial^2 u}{\partial z^2}.$$

We have

$$\frac{\partial q}{\partial \tau} = \frac{\partial^2 q}{\partial y^2} - \Psi(x, \tau) \frac{\partial q}{\partial y}, \quad \Psi(x, \tau) = \Phi_{\bar{\rho}}(x, -\log(\alpha(\tau)))\alpha(\tau), \quad (2)$$

Let us absorb the drift in the time derivative with the variable

$$z = y - \int_0^\tau \Psi(x, \eta) \, d\eta.$$

Then u solves

$$\frac{\partial u}{\partial \tau} = \frac{\partial^2 u}{\partial z^2}.$$

Oh! It looks **easy** again :) .

We have

$$\frac{\partial q}{\partial \tau} = \frac{\partial^2 q}{\partial y^2} - \Psi(x, \tau) \frac{\partial q}{\partial y}, \quad \Psi(x, \tau) = \Phi_{\bar{\rho}}(x, -\log(\alpha(\tau)))\alpha(\tau), \quad (2)$$

Let us absorb the drift in the time derivative with the variable

$$z = y - \int_0^\tau \Psi(x, \eta) d\eta.$$

Then u solves

$$\frac{\partial u}{\partial \tau} = \frac{\partial^2 u}{\partial z^2}.$$

Oh! It looks **easy** again :) . **Wait a minute...**

We have

$$\frac{\partial q}{\partial \tau} = \frac{\partial^2 q}{\partial y^2} - \Psi(x, \tau) \frac{\partial q}{\partial y}, \quad \Psi(x, \tau) = \Phi_{\bar{\rho}}(x, -\log(\alpha(\tau)))\alpha(\tau), \quad (2)$$

Let us absorb the drift in the time derivative with the variable

$$z = y - \int_0^\tau \Psi(x, \eta) d\eta.$$

Then u solves

$$\frac{\partial u}{\partial \tau} = \frac{\partial^2 u}{\partial z^2}.$$

Oh! It looks **easy** again :) . **Wait a minute...** Oh.

We have

$$\frac{\partial q}{\partial \tau} = \frac{\partial^2 q}{\partial y^2} - \Psi(x, \tau) \frac{\partial q}{\partial y}, \quad \Psi(x, \tau) = \Phi_{\bar{\rho}}(x, -\log(\alpha(\tau)))\alpha(\tau), \quad (2)$$

Let us absorb the drift in the time derivative with the variable

$$z = y - \int_0^\tau \Psi(x, \eta) \, d\eta.$$

Then u solves

$$\frac{\partial u}{\partial \tau} = \frac{\partial^2 u}{\partial z^2}.$$

Oh! It looks **easy** again :) . **Wait a minute...** Oh. Oh no.

What have we done

We forgot the boundary conditions.

What have we done

We forgot the boundary conditions. Define u by $u(x, z, \tau) = q(x, y, \tau)$ and denote

$$\gamma(x, \tau) = - \int_0^\tau \Psi(x, \eta) \, d\eta, \quad \bar{u}(x, \tau) = \int_{\gamma(x, \tau)}^{+\infty} zu(x, z, \tau) \, dz.$$

What have we done

We forgot the boundary conditions. Define u by $u(x, z, \tau) = q(x, y, \tau)$ and denote

$$\gamma(x, \tau) = - \int_0^\tau \Psi(x, \eta) d\eta, \quad \bar{u}(x, \tau) = \int_{\gamma(x, \tau)}^{+\infty} zu(x, z, \tau) dz.$$

$$\begin{aligned} \frac{\partial u}{\partial \tau}(x, z, \tau) &= \frac{\partial^2 u}{\partial z^2}(x, z, \tau), & z \in (\gamma(x, \tau), +\infty), \\ \gamma(x, \tau) &= - \int_0^\tau \Psi(x, \eta) d\eta, \\ \frac{\partial u}{\partial y}(x, \gamma(x, \tau), \tau) &= \Psi(x, \tau)u(x, \gamma(x, \tau), \tau), \\ \Psi(x, \tau) &= \Phi(\alpha(\tau)W * [\bar{u}(x, \tau) - \gamma(x, \tau)] + B)\alpha(\tau), \end{aligned}$$

What have we done

We forgot the boundary conditions. Define u by $u(x, z, \tau) = q(x, y, \tau)$ and denote

$$\gamma(x, \tau) = - \int_0^\tau \Psi(x, \eta) d\eta, \quad \bar{u}(x, \tau) = \int_{\gamma(x, \tau)}^{+\infty} zu(x, z, \tau) dz.$$

$$\begin{aligned} \frac{\partial u}{\partial \tau}(x, z, \tau) &= \frac{\partial^2 u}{\partial z^2}(x, z, \tau), & z \in (\gamma(x, \tau), +\infty), \\ \gamma(x, \tau) &= - \int_0^\tau \Psi(x, \eta) d\eta, \\ \frac{\partial u}{\partial y}(x, \gamma(x, \tau), \tau) &= \Psi(x, \tau)u(x, \gamma(x, \tau), \tau), \\ \Psi(x, \tau) &= \Phi(\alpha(\tau)W * [\bar{u}(x, \tau) - \gamma(x, \tau)] + B)\alpha(\tau), \end{aligned}$$

This is **still not** an easy problem :(.

Did we make any progress?

$$\frac{\partial \rho}{\partial t} = -\frac{\partial}{\partial s} \left(\left[\Phi_{\bar{\rho}}(\mathbf{x}, t) - s \right] \rho \right) + \sigma \frac{\partial^2 \rho}{\partial s^2}, \quad (3)$$

$$\Phi_{\bar{\rho}}(\mathbf{x}, t) = \Phi(W * \bar{\rho}(\mathbf{x}, t) + B), \quad \bar{\rho}(\mathbf{x}, t) = \int_0^\infty s \rho(\mathbf{x}, s, t) \, ds, \quad (4)$$

$$\Phi_{\bar{\rho}}(\mathbf{x}) \rho(\mathbf{x}, 0, t) - \sigma \frac{\partial \rho}{\partial s}(\mathbf{x}, 0, t) = 0. \quad (5)$$

Did we make any progress?

$$\frac{\partial \rho}{\partial t} = -\frac{\partial}{\partial s} \left([\Phi_{\bar{\rho}}(\mathbf{x}, t) - s] \rho \right) + \sigma \frac{\partial^2 \rho}{\partial s^2}, \quad (3)$$

$$\Phi_{\bar{\rho}}(\mathbf{x}, t) = \Phi(W * \bar{\rho}(\mathbf{x}, t) + B), \quad \bar{\rho}(\mathbf{x}, t) = \int_0^\infty s \rho(\mathbf{x}, s, t) \, ds, \quad (4)$$

$$\Phi_{\bar{\rho}}(\mathbf{x}) \rho(\mathbf{x}, 0, t) - \sigma \frac{\partial \rho}{\partial s}(\mathbf{x}, 0, t) = 0. \quad (5)$$

Change variables to obtain

$$\begin{aligned} \frac{\partial u}{\partial \tau}(x, z, \tau) &= \frac{\partial^2 u}{\partial z^2}(x, z, \tau), & z &\in (\gamma(x, \tau), +\infty), \\ \gamma(x, \tau) &= -\int_0^\tau \Psi(x, \eta) d\eta, \\ \frac{\partial u}{\partial y}(x, \gamma(x, \tau), \tau) &= \Psi(x, \tau) u(x, \gamma(x, \tau), \tau), \\ \Psi(x, \tau) &= \Phi(\alpha(\tau) W * [\bar{u}(x, \tau) - \gamma(x, \tau)] + B) \alpha(\tau), \end{aligned}$$

Solve the easy part at least

$$\frac{\partial u}{\partial \tau}(x, z, \tau) = \frac{\partial^2 u}{\partial z^2}(x, z, \tau), \quad z \in (\gamma(x, \tau), +\infty).$$

In order to obtain a Duhamel formula for u , we use the heat kernel

$$G(z, \tau, \xi, \eta) = \frac{1}{\sqrt{4\pi(\tau - \eta)}} e^{-\frac{(z - \xi)^2}{4(\tau - \eta)}}.$$

Solve the easy part at least

$$\frac{\partial u}{\partial \tau}(x, z, \tau) = \frac{\partial^2 u}{\partial z^2}(x, z, \tau), \quad z \in (\gamma(x, \tau), +\infty).$$

In order to obtain a Duhamel formula for u , we use the heat kernel

$$G(z, \tau, \xi, \eta) = \frac{1}{\sqrt{4\pi(\tau - \eta)}} e^{-\frac{(z - \xi)^2}{4(\tau - \eta)}}.$$

This kernel satisfies the Green identity

$$\frac{\partial}{\partial \xi} \left(G \frac{\partial u}{\partial \xi} - u \frac{\partial G}{\partial \xi} \right) - \frac{\partial}{\partial \eta} (Gu) = 0.$$

Solve the easy part at least

$$\frac{\partial u}{\partial \tau}(x, z, \tau) = \frac{\partial^2 u}{\partial z^2}(x, z, \tau), \quad z \in (\gamma(x, \tau), +\infty).$$

In order to obtain a Duhamel formula for u , we use the heat kernel

$$G(z, \tau, \xi, \eta) = \frac{1}{\sqrt{4\pi(\tau - \eta)}} e^{-\frac{(z - \xi)^2}{4(\tau - \eta)}}.$$

This kernel satisfies the Green identity

$$\frac{\partial}{\partial \xi} \left(G \frac{\partial u}{\partial \xi} - u \frac{\partial G}{\partial \xi} \right) - \frac{\partial}{\partial \eta} (Gu) = 0.$$

For each $x \in \mathbb{T}^d$, integrate on $(\gamma(x, \eta), +\infty)$ and then on $(0, \tau)$:

$$\begin{aligned} \int_0^\tau \int_{\gamma(x, \eta)}^{+\infty} \frac{\partial}{\partial \xi} \left(G \frac{\partial u}{\partial \xi} \right) d\xi d\eta - \int_0^\tau \int_{\gamma(x, \eta)}^{+\infty} \frac{\partial}{\partial \xi} \left(u \frac{\partial G}{\partial \xi} \right) d\xi d\eta \\ - \int_0^\tau \int_{\gamma(x, \eta)}^{+\infty} \frac{\partial}{\partial \eta} (Gu) d\xi d\eta = 0. \end{aligned}$$

Solve the easy part at least

$$\frac{\partial u}{\partial \tau}(x, z, \tau) = \frac{\partial^2 u}{\partial z^2}(x, z, \tau), \quad z \in (\gamma(x, \tau), +\infty).$$

In order to obtain a Duhamel formula for u , we use the heat kernel

$$G(z, \tau, \xi, \eta) = \frac{1}{\sqrt{4\pi(\tau - \eta)}} e^{-\frac{(z - \xi)^2}{4(\tau - \eta)}}.$$

For each $x \in \mathbb{T}^d$, integrate on $(\gamma(x, \eta), +\infty)$ and then on $(0, \tau)$:

$$\underbrace{\int_0^\tau \int_{\gamma(x, \eta)}^{+\infty} \frac{\partial}{\partial \xi} \left(G \frac{\partial u}{\partial \xi} \right) d\xi d\eta}_I - \underbrace{\int_0^\tau \int_{\gamma(x, \eta)}^{+\infty} \frac{\partial}{\partial \xi} \left(u \frac{\partial G}{\partial \xi} \right) d\xi d\eta}_{II} - \underbrace{\int_0^\tau \int_{\gamma(x, \eta)}^{+\infty} \frac{\partial}{\partial \eta} (Gu) d\xi d\eta}_{III} = 0.$$

Solve the easy part at least

$$\frac{\partial u}{\partial \tau}(x, z, \tau) = \frac{\partial^2 u}{\partial z^2}(x, z, \tau), \quad z \in (\gamma(x, \tau), +\infty).$$

Computing *I*, *II*, *III* we get

$$u(x, z, \tau) = \int_0^{+\infty} G(z, \tau, \xi, 0) u^0(x, \xi) d\xi \quad (6)$$

$$+ \int_0^\tau \frac{\partial G}{\partial \xi}(z, \tau, \gamma(x, \eta), \eta) u(x, \gamma(x, \eta), \eta) d\eta. \quad (7)$$

Time evolution problem

Define

$$v(x, \tau) = u(x, \gamma(x, \tau), \tau).$$

And use the heat Kernel to find a closed system

$$\begin{cases} v(x, \tau) &= F_v[v, \gamma, \bar{u}](x, \tau) & \text{boundary value,} \\ \gamma(x, \tau) &= F_\gamma[v, \gamma, \bar{u}](x, \tau) & \text{boundary position,} \\ \bar{u}(x, \tau) &= F_{\bar{u}}[v, \gamma, \bar{u}](x, \tau) & \text{average.} \end{cases}$$

Then, painfully apply a Fixed point argument to the system.

Time evolution problem

Define

$$v(x, \tau) = u(x, \gamma(x, \tau), \tau).$$

And use the heat Kernel to find a closed system

$$\begin{cases} v(x, \tau) &= F_v[v, \gamma, \bar{u}](x, \tau) & \text{boundary value,} \\ \gamma(x, \tau) &= F_\gamma[v, \gamma, \bar{u}](x, \tau) & \text{boundary position,} \\ \bar{u}(x, \tau) &= F_{\bar{u}}[v, \gamma, \bar{u}](x, \tau) & \text{average.} \end{cases}$$

Then, painfully apply a Fixed point argument to the system.

→ Local existence and regularity of the equation.

Time evolution problem

Define

$$v(x, \tau) = u(x, \gamma(x, \tau), \tau).$$

And use the heat Kernel to find a closed system

$$\begin{cases} v(x, \tau) &= F_v[v, \gamma, \bar{u}](x, \tau) & \text{boundary value,} \\ \gamma(x, \tau) &= F_\gamma[v, \gamma, \bar{u}](x, \tau) & \text{boundary position,} \\ \bar{u}(x, \tau) &= F_{\bar{u}}[v, \gamma, \bar{u}](x, \tau) & \text{average.} \end{cases}$$

Then, painfully apply a Fixed point argument to the system.

→ Local existence and regularity of the equation.

→ Global existence can be obtained with uniform bounds on v , γ and \bar{u} .

Thank you !

